@prefix rdfs:      <http://www.w3.org/2000/01/rdf-schema#> .
@prefix jdcrp:     <https://graph.jdcrp.org/schema#> .
@prefix shape:     <https://graph.jdcrp.org/schema#> .
@prefix xsd:       <http://www.w3.org/2001/XMLSchema#> .
@prefix rdf:       <http://www.w3.org/1999/02/22-rdf-syntax-ns#> .

jdcrp:Person
	a               rdfs:Class ;
	rdfs:subClassOf jdcrp:LegalEntity .

# Note: If you only have a combined name, use "name" inherited from SourceLegalEntity

jdcrp:firstName
	a            rdf:Property ;
	rdfs:domain  jdcrp:Person ;
	rdfs:range   xsd:string ;
	rdfs:label   "first name" ;
	rdfs:comment "The first name of this person" .

jdcrp:lastName
	a            rdf:Property ;
	rdfs:domain  jdcrp:Person ;
	rdfs:range   xsd:string ;
	rdfs:label   "last name" ;
	rdfs:comment "The last name of this person" .

jdcrp:pseudonym
	a            rdf:Property ;
	rdfs:domain  jdcrp:Person ;
	rdfs:range   xsd:string ;
	rdfs:label   "pseudonym" ;
	rdfs:comment "The pseudonym, nickname or artist's name of this person" .

jdcrp:historyDescription
	a            rdf:Property ;
	rdfs:domain  jdcrp:Person ;
	rdfs:range   xsd:string ;
	rdfs:label   "history description" ;
	rdfs:comment "An unstructured, textual description of this person's history" .

jdcrp:birthDate
	a            rdf:Property ;
	rdfs:domain  jdcrp:Person ;
	rdfs:range   xsd:string ;
	rdfs:label   "birth date" ;
	rdfs:comment "The date of birth of this person, possibly as an unstructured string" .

jdcrp:structuredBirthDate
	a            rdf:Property ;
	rdfs:domain  jdcrp:Person ;
	rdfs:range   xsd:date ;
	rdfs:label   "structured birth date" ;
	rdfs:comment "The date of birth of this person, as a structured date" .

jdcrp:bornInLocation
	a            rdf:Property ;
	rdfs:domain  jdcrp:Person ;
	rdfs:range   jdcrp:Location ;
	rdfs:label   "birth place" ;
	rdfs:comment "The location where this person was born" .

jdcrp:deathDate
	a            rdf:Property ;
	rdfs:domain  jdcrp:Person ;
	rdfs:range   xsd:string ;
	rdfs:label   "death date" ;
	rdfs:comment "The date of death of this person, possibly as an unstructured string" .

jdcrp:lifetime
	a            rdf:Property ;
	rdfs:domain  jdcrp:Person ;
	rdfs:range   xsd:string ;
	rdfs:label   "lifetime" ;
	rdfs:comment "The time at which this person was generally alive or active, possibly as an unstructured string" .

jdcrp:structuredDeathDate
	a            rdf:Property ;
	rdfs:domain  jdcrp:Person ;
	rdfs:range   xsd:date ;
	rdfs:label   "structured death date" ;
	rdfs:comment "The date of death of this person, as a structured date" .

jdcrp:diedInLocation
	a            rdf:Property ;
	rdfs:domain  jdcrp:Person ;
	rdfs:range   jdcrp:Location ;
	rdfs:label   "death place" ;
	rdfs:comment "The location where this person died" .
