@prefix rdf:   <http://www.w3.org/1999/02/22-rdf-syntax-ns#> .
@prefix xsd:   <http://www.w3.org/2001/XMLSchema#> .
@prefix rdfs:  <http://www.w3.org/2000/01/rdf-schema#> .
@prefix jdcrp: <https://graph.jdcrp.org/schema#> .

jdcrp:Location
	a               rdfs:Class ;
	rdfs:subClassOf jdcrp:Entity .

jdcrp:partOf
	a            rdf:Property ;
	rdfs:domain  jdcrp:Location ;
	rdfs:range   jdcrp:Location ;
	rdfs:label   "partOf" ;
	rdfs:comment "Another location that this location is entirely part of" .

jdcrp:description
	a            rdf:Property ;
	rdfs:domain  jdcrp:Location ;
	rdfs:range   xsd:string ;
	rdfs:label   "description" ;
	rdfs:comment "A textual description of the location" .

jdcrp:street
	a            rdf:Property ;
	rdfs:domain  jdcrp:Location ;
	rdfs:range   xsd:string ;
	rdfs:label   "street" ;
	rdfs:comment "The street part of this location's address, including house number, as a string" .

jdcrp:city
	a            rdf:Property ;
	rdfs:domain  jdcrp:Location ;
	rdfs:range   xsd:string ;
	rdfs:label   "city" ;
	rdfs:comment "The city part of this location's address, as a string" .

jdcrp:region
	a            rdf:Property ;
	rdfs:domain  jdcrp:Location ;
	rdfs:range   xsd:string ;
	rdfs:label   "region" ;
	rdfs:comment "The region part of this location's address, as a string" .

jdcrp:country
	a            rdf:Property ;
	rdfs:domain  jdcrp:Location ;
	rdfs:range   xsd:string ;
	rdfs:label   "country" ;
	rdfs:comment "The country part of this location's address, as a string" .

jdcrp:latitude
	a            rdf:Property ;
	rdfs:domain  jdcrp:Location ;
	rdfs:range   xsd:decimal ;
	rdfs:label   "latitude" ;
	rdfs:comment "The known latitude of this location, according to the source." .

jdcrp:longitude
	a            rdf:Property ;
	rdfs:domain  jdcrp:Location ;
	rdfs:range   xsd:decimal ;
	rdfs:label   "longitude" ;
	rdfs:comment "The known longitude of this location, according to the source." .
