@prefix rdf:   <http://www.w3.org/1999/02/22-rdf-syntax-ns#> .
@prefix xsd:   <http://www.w3.org/2001/XMLSchema#> .
@prefix rdfs:  <http://www.w3.org/2000/01/rdf-schema#> .
@prefix jdcrp: <https://graph.jdcrp.org/schema#> .

jdcrp:TransferEvent
	a               rdfs:Class ;
	rdfs:subClassOf jdcrp:CulturalAssetEvent .

jdcrp:departureDate
	a            rdf:Property ;
	rdfs:domain  jdcrp:TransferEvent ;
	rdfs:range   xsd:string ;
	rdfs:label   "departure date" ;
	rdfs:comment "The date the cultural asset was departured from the original location" .

jdcrp:structuredDepartureDate
	a            rdf:Property ;
	rdfs:domain  jdcrp:TransferEvent ;
	rdfs:range   xsd:string ;
	rdfs:label   "structured departure date" ;
	rdfs:comment "Structured version of departure date" .

jdcrp:arrivalDate
	a            rdf:Property ;
	rdfs:domain  jdcrp:TransferEvent ;
	rdfs:range   xsd:string ;
	rdfs:label   "arrival date" ;
	rdfs:comment "The date the cultural asset arrived at the destination" .

jdcrp:structuredArrivalDate
	a            rdf:Property ;
	rdfs:domain  jdcrp:TransferEvent ;
	rdfs:range   xsd:string ;
	rdfs:label   "structured arrival date" ;
	rdfs:comment "Structured version of arrival date" .

jdcrp:physicalDescriptionBefore
	a            rdf:Property ;
	rdfs:domain  jdcrp:TransferEvent ;
	rdfs:range   xsd:string ;
	rdfs:label   "physical description before" ;
	rdfs:comment "The physical description of the cultural asset before the transferration" .

jdcrp:physicalDescriptionAfter
	a            rdf:Property ;
	rdfs:domain  jdcrp:TransferEvent ;
	rdfs:range   xsd:string ;
	rdfs:label   "physical description after" ;
	rdfs:comment "The physical description of the cultural asset after the transferration" .

jdcrp:fromLocation
	a            rdf:Property ;
	rdfs:domain  jdcrp:TransferEvent ;
	rdfs:range   jdcrp:Location ;
	rdfs:label   "from location" ;
	rdfs:comment "The origin location from which the cultural asset(s) were transferred" .

jdcrp:toLocation
	a            rdf:Property ;
	rdfs:domain  jdcrp:TransferEvent ;
	rdfs:range   jdcrp:Location ;
	rdfs:label   "to location" ;
	rdfs:comment "The destination location to which the cultural asset(s) were transferred" .

jdcrp:fromCollection
	a            rdf:Property ;
	rdfs:domain  jdcrp:TransferEvent ;
	rdfs:range   jdcrp:Collection ;
	rdfs:label   "from collection" ;
	rdfs:comment "The collection from which the cultural asset(s) originated" .

jdcrp:toCollection
	a            rdf:Property ;
	rdfs:domain  jdcrp:TransferEvent ;
	rdfs:range   jdcrp:Collection ;
	rdfs:label   "to collection" ;
	rdfs:comment "The collection to which the cultural asset(s) were transferred" .

jdcrp:byLegalEntity
	a            rdf:Property ;
	rdfs:domain  jdcrp:TransferEvent ;
	rdfs:range   jdcrp:LegalEntity ;
	rdfs:label   "by legal entity" ;
	rdfs:comment "The legal entity who was responsible for the transferration" .

jdcrp:identifiedBy
	a            rdf:Property ;
	rdfs:domain  jdcrp:TransferEvent ;
	rdfs:range   jdcrp:LegalEntity ;
	rdfs:label   "identified by" ;
	rdfs:comment "The legal entities who were responsible for the identification of the cultural asset at destination" .

jdcrp:possessorBefore
	a            rdf:Property ;
	rdfs:domain  jdcrp:TransferEvent ;
	rdfs:range   jdcrp:LegalEntity ;
	rdfs:label   "possessor before" ;
	rdfs:comment "The legal entity who possessed the cultural asset before transferration" .

jdcrp:possessorAfter
	a            rdf:Property ;
	rdfs:domain  jdcrp:TransferEvent ;
	rdfs:range   jdcrp:LegalEntity ;
	rdfs:label   "possessor after" ;
	rdfs:comment "The legal entity who possessed the cultural asset after transferration" .
