@prefix rdf:   <http://www.w3.org/1999/02/22-rdf-syntax-ns#> .
@prefix xsd:   <http://www.w3.org/2001/XMLSchema#> .
@prefix rdfs:  <http://www.w3.org/2000/01/rdf-schema#> .
@prefix jdcrp: <https://graph.jdcrp.org/schema#> .

jdcrp:CulturalAsset
	a               rdfs:Class ;
	rdfs:subClassOf jdcrp:Entity .

jdcrp:title
	a            rdf:Property ;
	rdfs:domain  jdcrp:CulturalAsset ;
	rdfs:range   xsd:string ;
	rdfs:label   "title" ;
	rdfs:comment "The title of this cultural asset" .

jdcrp:collectedIn
	a            rdf:Property ;
	rdfs:domain  jdcrp:CulturalAsset ;
	rdfs:range   jdcrp:Collection ;
	rdfs:label   "collected in" ;
	rdfs:comment "The collection of this cultural asset" .

jdcrp:classifiedAs
	a            rdf:Property ;
	rdfs:domain  jdcrp:CulturalAsset ;
	rdfs:range   jdcrp:Classification ;
	rdfs:label   "classified as" ;
	rdfs:comment "The classification of this cultural asset" .

jdcrp:consistsOfMaterial
	a            rdf:Property ;
	rdfs:domain  jdcrp:CulturalAsset ;
	rdfs:range   jdcrp:Material ;
	rdfs:label   "consists of material" ;
	rdfs:comment "The material type that this cultural asset is made of" .

jdcrp:locatedIn
	a            rdf:Property ;
	rdfs:domain  jdcrp:CulturalAsset ;
	rdfs:range   jdcrp:Location ;
	rdfs:label   "located in" ;
	rdfs:comment "The location where this cultural asset is located" .

jdcrp:createdInLocation
	a            rdf:Property ;
	rdfs:domain  jdcrp:CulturalAsset ;
	rdfs:range   jdcrp:Location ;
	rdfs:label   "created in location" ;
	rdfs:comment "The location where this cultural asset was created" .

jdcrp:createdBy
	a            rdf:Property ;
	rdfs:domain  jdcrp:CulturalAsset ;
	rdfs:range   jdcrp:LegalEntity ;
	rdfs:label   "created by" ;
	rdfs:comment "The person who created this cultural asset" .

jdcrp:creationDate
	a            rdf:Property ;
	rdfs:domain  jdcrp:CulturalAsset ;
	rdfs:range   xsd:string ;
	rdfs:label   "creation date" ;
	rdfs:comment "The date when this cultural asset was created, possibly as an unstructured string" .

jdcrp:structuredCreationDate
	a            rdf:Property ;
	rdfs:domain  jdcrp:CulturalAsset ;
	rdfs:range   xsd:date ;
	rdfs:label   "structured creation date" ;
	rdfs:comment "The date when this cultural asset was created, as a structured date" .

jdcrp:measurements
	a            rdf:Property ;
	rdfs:domain  jdcrp:CulturalAsset ;
	rdfs:range   xsd:string ;
	rdfs:label   "measurements" ;
	rdfs:comment "The measurements of this cultural asset, possibly as an unstructured string" .

jdcrp:weight
	a            rdf:Property ;
	rdfs:domain  jdcrp:CulturalAsset ;
	rdfs:range   xsd:string ;
	rdfs:label   "weight" ;
	rdfs:comment "The weight of this cultural asset, possibly as an unstructured string" .

jdcrp:annotation
	a            rdf:Property ;
	rdfs:domain  jdcrp:CulturalAsset ;
	rdfs:range   xsd:string ;
	rdfs:label   "annotation" ;
	rdfs:comment "Any annotations related to this cultural asset" .

jdcrp:identifyingMarks
	a            rdf:Property ;
	rdfs:domain  jdcrp:CulturalAsset ;
	rdfs:range   xsd:string ;
	rdfs:label   "identifying marks" ;
	rdfs:comment "A textual description of any identifying marks found found on / specific to this cultural asset" .

jdcrp:archivalSourceDescription
	a            rdf:Property ;
	rdfs:domain  jdcrp:CulturalAsset ;
	rdfs:range   xsd:string ;
	rdfs:label   "archival source description" ;
	rdfs:comment "Textual info on where this cultural asset was exactly discovered, e.g. the Bundesarchiv number" .

jdcrp:physicalDescription
	a            rdf:Property ;
	rdfs:domain  jdcrp:CulturalAsset ;
	rdfs:range   xsd:string ;
	rdfs:label   "physical description" ;
	rdfs:comment "A textual description of the physical appearance of this cultural asset" .

jdcrp:physicalConditionDescription
	a            rdf:Property ;
	rdfs:domain  jdcrp:CulturalAsset ;
	rdfs:range   xsd:string ;
	rdfs:label   "physical condition description" ;
	rdfs:comment "A textual description of the physical condition of this cultural asset" .

jdcrp:provenanceDescription
	a            rdf:Property ;
	rdfs:domain  jdcrp:CulturalAsset ;
	rdfs:range   xsd:string ;
	rdfs:label   "provenance description" ;
	rdfs:comment "A textual description of the provenance of this cultural asset" .

jdcrp:preConfiscationHistoryDescription
	a            rdf:Property ;
	rdfs:domain  jdcrp:CulturalAsset ;
	rdfs:range   xsd:string ;
	rdfs:label   "pre-confiscation history description" ;
	rdfs:comment "A textual description of the history of this cultural asset before it was confiscated" .

jdcrp:postConfiscationHistoryDescription
	a            rdf:Property ;
	rdfs:domain  jdcrp:CulturalAsset ;
	rdfs:range   xsd:string ;
	rdfs:label   "post-confiscation history description" ;
	rdfs:comment "A textual description of the history of this cultural asset after it was confiscated" .

jdcrp:currentRemainDescription
	a            rdf:Property ;
	rdfs:domain  jdcrp:CulturalAsset ;
	rdfs:range   xsd:string ;
	rdfs:label   "current remain description" ;
	rdfs:comment "A textual description of the current state of this cultural asset" .

jdcrp:wccpNumber
	a            rdf:Property ;
	rdfs:domain  jdcrp:CulturalAsset ;
	rdfs:range   xsd:string ;
	rdfs:label   "wccp number" ;
	rdfs:comment "The wiesbaden central collection point number of this cultural asset, if applicable" .

jdcrp:marburgNumber
	a            rdf:Property ;
	rdfs:domain  jdcrp:CulturalAsset ;
	rdfs:range   xsd:string ;
	rdfs:label   "marburg number" ;
	rdfs:comment "The marburg central collection point number of this cultural asset, if applicable" .

jdcrp:munichNumber
	a            rdf:Property ;
	rdfs:domain  jdcrp:CulturalAsset ;
	rdfs:range   xsd:string ;
	rdfs:label   "munich number" ;
	rdfs:comment "The munich number of this cultural asset, if applicable" .

jdcrp:linzNumber
	a            rdf:Property ;
	rdfs:domain  jdcrp:CulturalAsset ;
	rdfs:range   xsd:string ;
	rdfs:label   "linz number" ;
	rdfs:comment "The linz number of this cultural asset, if applicable" .

jdcrp:errNumber
	a            rdf:Property ;
	rdfs:domain  jdcrp:CulturalAsset ;
	rdfs:range   xsd:string ;
	rdfs:label   "err number" ;
	rdfs:comment "The Einsatzstab Reichsleiter Rosenberg number of this cultural asset, if applicable" .

jdcrp:inventoryNumber
	a            rdf:Property ;
	rdfs:domain  jdcrp:CulturalAsset ;
	rdfs:range   xsd:string ;
	rdfs:label   "inventory number" ;
	rdfs:comment "The inventory number in the context of the Wiesbaden or Marburg Central collecting point" .

jdcrp:catalogNumber
	a            rdf:Property ;
	rdfs:domain  jdcrp:CulturalAsset ;
	rdfs:range   xsd:string ;
	rdfs:label   "catalog number" ;
	rdfs:comment "The catalog number in the context of the Wiesbaden or Marburg Central collecting point" .

jdcrp:negativeNumber
	a            rdf:Property ;
	rdfs:domain  jdcrp:CulturalAsset ;
	rdfs:range   xsd:string ;
	rdfs:label   "negative number" ;
	rdfs:comment "The negative number in the context of the Wiesbaden or Marburg Central collecting point" .

jdcrp:claimNumber
	a            rdf:Property ;
	rdfs:domain  jdcrp:CulturalAsset ;
	rdfs:range   xsd:string ;
	rdfs:label   "claim number" ;
	rdfs:comment "The claim number in the context of the Wiesbaden or Marburg Central collecting point" .

jdcrp:depictedInImage
	a            rdf:Property ;
	rdfs:domain  jdcrp:CulturalAsset ;
	rdfs:range   jdcrp:Image ;
	rdfs:label   "depicted in" ;
	rdfs:comment "An image of the physical cultural asset" .

jdcrp:referencedInCardImage
	a            rdf:Property ;
	rdfs:domain  jdcrp:CulturalAsset ;
	rdfs:range   jdcrp:Image ;
	rdfs:label   "referenced in card image" ;
	rdfs:comment "An image of the card this cultural asset is referenced in" .

jdcrp:referencedInCardImageFront
	a            rdf:Property ;
	rdfs:domain  jdcrp:CulturalAsset ;
	rdfs:range   jdcrp:Image ;
	rdfs:label   "referenced in card image front" ;
	rdfs:comment "An image of the front of a card this cultural asset is referenced in" .

jdcrp:referencedInCardImageBack
	a            rdf:Property ;
	rdfs:domain  jdcrp:CulturalAsset ;
	rdfs:range   jdcrp:Image ;
	rdfs:label   "referenced in card image back" ;
	rdfs:comment "An image of the back of a card this card this cultural asset is referenced in" .

jdcrp:informationOnImages
	a            rdf:Property ;
	rdfs:domain  jdcrp:CulturalAsset ;
	rdfs:range   xsd:string ;
	rdfs:label   "information on images" ;
	rdfs:comment "Information on the images of this cultural asset e.g. links to negatives" .

jdcrp:copiesOfCard
	a            rdf:Property ;
	rdfs:domain  jdcrp:CulturalAsset ;
	rdfs:range   xsd:string ;
	rdfs:label   "copies of card" ;
	rdfs:comment "The number of copies of this property card" .

jdcrp:bibliography
	a            rdf:Property ;
	rdfs:domain  jdcrp:CulturalAsset ;
	rdfs:range   xsd:string ;
	rdfs:label   "bibliography" ;
	rdfs:comment "Related literature to this cultural asset " .

jdcrp:bundesarchivBand
	a            rdf:Property ;
	rdfs:domain  jdcrp:CulturalAsset ;
	rdfs:range   xsd:string ;
	rdfs:label   "bundesarchiv band" ;
	rdfs:comment "The band number of the Bundesarchiv where this cultural asset is referenced" .

jdcrp:bundesarchivSignature
	a            rdf:Property ;
	rdfs:domain  jdcrp:CulturalAsset ;
	rdfs:range   xsd:string ;
	rdfs:label   "bundesarchiv signature" ;
	rdfs:comment "The signature of the Bundesarchiv where this cultural asset is referenced" .

jdcrp:bundesarchivTitle
	a            rdf:Property ;
	rdfs:domain  jdcrp:CulturalAsset ;
	rdfs:range   xsd:string ;
	rdfs:label   "bundesarchiv title" ;
	rdfs:comment "The title of the Bundesarchiv where this cultural asset is referenced" .

jdcrp:bundesarchivStartDate
	a            rdf:Property ;
	rdfs:domain  jdcrp:CulturalAsset ;
	rdfs:range   xsd:string ;
	rdfs:label   "bundesarchiv start date" ;
	rdfs:comment "The start date of the duration in Bundesarchiv" .

jdcrp:bundesarchivEndDate
	a            rdf:Property ;
	rdfs:domain  jdcrp:CulturalAsset ;
	rdfs:range   xsd:string ;
	rdfs:label   "bundesarchiv end date" ;
	rdfs:comment "The end date of the duration in Bundesarchiv" .

jdcrp:bundesarchivPropertyCardFileNameFront
	a            rdf:Property ;
	rdfs:domain  jdcrp:CulturalAsset ;
	rdfs:range   xsd:string ;
	rdfs:label   "bundesarchiv property card file name front" ;
	rdfs:comment "The file name of the front of the property card in the Bundesarchiv" .

jdcrp:bundesarchivPropertyCardFileNameBack
	a            rdf:Property ;
	rdfs:domain  jdcrp:CulturalAsset ;
	rdfs:range   xsd:string ;
	rdfs:label   "bundesarchiv property card file name back" ;
	rdfs:comment "The file name of the back of the property card in the Bundesarchiv" .

jdcrp:shelfNumber
	a            rdf:Property ;
	rdfs:domain  jdcrp:CulturalAsset ;
	rdfs:range   xsd:string ;
	rdfs:label   "shelf number" ;
	rdfs:comment "The shelf number of this cultural asset in the Collection Point" .
